x86/LinkingProp.v
@@ -1,0 +1,195 @@
+Require Import Coqlib Integers AST Maps.
+Require Import Linking.
+Import ListNotations.
+
+Set Implicit Arguments.
+
+Lemma is_def_internal_dec' : forall (F V:Type) (f:F -> bool) (def: option (globdef F V)),
+    {is_def_internal f def = true} + {is_def_internal f def <> true}.
+Proof.
+  decide equality.
+Qed.
+
+Lemma is_def_internal_dec : forall (F V:Type) (f:F -> bool) (def: option (globdef F V)),
+    {is_def_internal f def = true} + {is_def_internal f def = false}.
+Proof.
+  intros F V f def.
+  generalize (is_def_internal_dec' f def).
+  intro H.
+  inv H. auto.
+  rewrite not_true_iff_false in H0. auto.
+Qed.  
+
+Lemma link_fundef_inv1 : forall (F:Type) (f: AST.fundef F) f' e, 
+    link_fundef f (External e) = Some f' -> f = f'.
+Proof.
+  intros F f f' e LINK.
+  destruct f. simpl in *. destruct e; try congruence.
+  simpl in LINK. destruct (external_function_eq e0 e); congruence.
+Qed.
+
+Lemma link_extern_fundef_inv: forall (F:Type) 
+                                (f f' f'': AST.fundef F),
+    is_fundef_internal f = false ->
+    link f' f = Some f'' -> 
+    f' = f''.
+Proof.
+  intros F f f' f'' FINT LINK.
+  unfold link in LINK. 
+  Transparent Linker_fundef.
+  unfold Linker_fundef in LINK.
+  destruct f; simpl in *. congruence.
+  simpl in LINK.
+  apply link_fundef_inv1 in LINK. auto.
+Qed.
+
+Lemma link_external_fundefs: forall (F: Type) (f1 f2 f: AST.fundef F), 
+    is_fundef_internal f1 = false ->
+    is_fundef_internal f2 = false ->
+    link_fundef f1 f2 = Some f ->
+    is_fundef_internal f = false.
+Proof.
+  intros F f1 f2 f INT1 INT2 LINK.
+  generalize (link_extern_fundef_inv f2 f1 INT2 LINK).
+  intros. subst. auto.
+Qed.
+
+
+Lemma link_extern_gfundef_inv: forall (F V:Type) (LV: Linker V)
+                             (f: AST.fundef F) (g g': (globdef (AST.fundef F) V)),
+    is_fundef_internal f = false ->
+    link g (Gfun f) = Some g' -> 
+    g = g'.
+Proof.
+  intros F V LV f g g' INT LINK.
+  destruct g. 
+  - unfold link in LINK. 
+    Transparent Linker_def.
+    unfold Linker_def in LINK.
+    simpl in LINK. destruct (link_fundef f0 f) eqn:LINKF; try congruence.
+    inv LINK.
+    generalize (link_extern_fundef_inv _ _ INT LINKF).
+    intros. subst.
+    auto.
+  - simpl in LINK. congruence.
+Qed.
+
+Lemma link_external_varinit: forall (V: Type) (LV: Linker V)(v1 v2: globvar V) l, 
+    is_var_internal v1 = false ->
+    is_var_internal v2 = false ->
+    link_varinit (gvar_init v1) (gvar_init v2) = Some l ->
+    classify_init l <> Init_definitive l.
+Proof.
+  intros V LV v1 v2 l INT1 INT2 LINK.
+  unfold link_varinit in LINK.
+  unfold is_var_internal in *.
+  destr_in LINK. inv LINK.
+  destr_in INT2.
+  destr_in INT2. inv LINK. congruence.
+  destr_in LINK; try congruence.
+  inv LINK. congruence.
+Qed.
+
+Lemma link_external_vars: forall (V: Type) (LV: Linker V)(v1 v2 v: globvar V), 
+    is_var_internal v1 = false ->
+    is_var_internal v2 = false ->
+    link v1 v2 = Some v ->
+    is_var_internal v = false.
+Proof.
+  intros V LV v1 v2 v INT1 INT2 LINK.
+  unfold link in LINK.
+  Transparent Linker_vardef.
+  unfold Linker_vardef in LINK.
+  unfold link_vardef in LINK.
+  destr_in LINK. destr_in LINK.
+  destr_in LINK. inv LINK.
+  unfold is_var_internal. simpl.
+  unfold link in Heqo0.
+  Transparent Linker_varinit.
+  unfold Linker_varinit in Heqo0.
+  generalize (link_external_varinit _ v1 v2 INT1 INT2 Heqo0).
+  intros. destruct (classify_init l); auto.
+  congruence.
+Qed.
+
+
+(* Lemma link_varinit_nil: forall i1 i2, link i1 nil = Some i2 -> i1 = i2. *)
+(* Proof. *)
+(*   intros i1 i2 LINK. *)
+(*   unfold link in LINK. *)
+(*   Transparent Linker_varinit. *)
+(*   unfold Linker_varinit in LINK.  *)
+(*   unfold link_varinit in LINK. *)
+(*   destr_in LINK. simpl in *. inv LINK. auto. *)
+(*   simpl in *. inv LINK. auto. *)
+(* Qed. *)
+
+(* Lemma link_varinit_space: forall i1 i2 sz, *)
+(*     link i1 [Init_space sz] = Some i2 -> i1 = i2. *)
+(* Proof. *)
+(*   (* intros i1 i2 sz LINK. *) *)
+(*   (* unfold link in LINK. *) *)
+(*   (* Transparent Linker_varinit. *) *)
+(*   (* unfold Linker_varinit in LINK. *) *)
+(*   (* unfold link_varinit in LINK.  *) *)
+(*   (* destruct i1. *) *)
+(*   (* - simpl in *. *) *)
+(*   (* destr_in LINK. simpl in *. inv LINK *) *)
+(*   Admitted. *)
+
+
+(* Lemma link_extern_varinit_inv: forall (V:Type) (v:globvar V) i1 i2, *)
+(*     is_var_internal v = false -> *)
+(*     link i1 (gvar_init v) = Some i2 -> i1 = i2. *)
+(* Proof. *)
+(*   (* intros V v i1 i2 VINT LINK. *) *)
+(*   (* unfold is_var_internal in VINT. *) *)
+(*   (* destruct (gvar_init v).  *) *)
+(*   (* -  *) *)
+
+
+
+(*   (* - destruct i; simpl in *; try congruence. *) *)
+(*   (*   destruct l; simpl in *. admit. *) *)
+(*   (*   congruence. *) *)
+(* Admitted. *)
+
+(* Lemma link_extern_var_inv: forall (V:Type) (LV:Linker V) *)
+(*                                 (v v' v'': globvar V), *)
+(*     is_var_internal v = false -> *)
+(*     link v' v = Some v'' ->  *)
+(*     gvar_init v' = gvar_init v''. *)
+(* Proof. *)
+(*   intros V LV v v' v'' VINT LINK. *)
+(*   unfold link in LINK.  *)
+(*   Transparent Linker_vardef. *)
+(*   unfold Linker_vardef in LINK. *)
+(*   unfold link_vardef in LINK. *)
+(*   destruct (link (gvar_info v') (gvar_info v)) eqn:LINK_INFO; try congruence. *)
+(*   destruct (link (gvar_init v') (gvar_init v)) eqn:LINK_INIT; try congruence. *)
+(*   destruct (eqb (gvar_readonly v') (gvar_readonly v) && eqb (gvar_volatile v') (gvar_volatile v)) eqn:EQB;  *)
+(*     try congruence. *)
+(*   inv LINK. simpl. *)
+(*   eapply link_extern_varinit_inv; eauto. *)
+(* Qed. *)
+
+(* Lemma link_extern_gvar_inv: forall (F V:Type) (LV: Linker V) *)
+(*                               (v: globvar V) (g g': (globdef (AST.fundef F) V)), *)
+(*     is_var_internal v = false -> *)
+(*     link g (Gvar v) = Some g' ->  *)
+(*     g = g'. *)
+(* Proof. *)
+(*   intros F V LV v g g' INT LINK. *)
+(*   destruct g.  *)
+(*   - unfold link in LINK.  *)
+(*     Transparent Linker_def. *)
+(*     unfold Linker_def in LINK. *)
+(*     simpl in LINK. congruence. *)
+(*   - simpl in LINK.  *)
+(*     destruct (link_vardef v0 v) eqn:LINKV; try congruence. *)
+(*     inv LINK. *)
+(*     generalize (link_extern_var_inv _ _ _ INT LINKV). *)
+(*     intros. subst. *)
+(*     auto. *)
+(*     Admitted. *)
+
